step 1: add serializer in spec until parse_nlist (included), all_bytes (excluded)

src/3d/prelude/EverParse3d.Prelude.fst
@@ -28,7 +28,45 @@ module U64 = FStar.UInt64
 // Parsers
 ////////////////////////////////////////////////////////////////////////////////
 
-let parser k t = LP.parser k t
+[@@erasable]
+noeq
+type full_parser (#nz:bool) (#wk: weak_kind) (k:parser_kind nz wk) (t:Type u#r) : Type u#r = {
+  pf_parser: LP.parser k t;
+  pf_serializer: LP.serializer pf_parser;
+}
+
+[@@erasable]
+noeq
+type parser (#nz:bool) (#wk: weak_kind) (k:parser_kind nz wk) (t:Type u#r) : Type u#r = {
+  p_serializable: (t -> GTot bool);
+  p_full_parser: full_parser k (LPC.parse_filter_refine p_serializable);
+}
+
+let mk_parser_gen
+  (#nz:bool) (#wk: weak_kind) (#k:parser_kind nz wk) (#t1:Type u#r)
+  (p1: full_parser k t1)
+  (#t2: Type u#r)
+  (ser: (t2 -> GTot bool))
+  (f12: (t1 -> GTot (LPC.parse_filter_refine ser)) { LPC.synth_injective f12 })
+  (f21: (LPC.parse_filter_refine ser -> GTot t1) { LPC.synth_inverse f12 f21 })
+: Tot (parser k t2)
+= {
+  p_serializable = ser;
+  p_full_parser = {
+    pf_parser = LPC.parse_synth p1.pf_parser f12;
+    pf_serializer = LPC.serialize_synth _ _ p1.pf_serializer f21 ();
+  }
+}
+
+let mk_parser
+  (#nz:bool) (#wk: weak_kind) (#k:parser_kind nz wk) (#t:Type u#r)
+  (p1: full_parser k t)
+: Tot (parser k t)
+= mk_parser_gen
+    p1
+    (fun _ -> true)
+    (fun x -> x)
+    (fun x -> x)
 
 let is_weaker_than #nz1 #wk1 (k:parser_kind nz1 wk1)
                    #nz2 #wk2 (k':parser_kind nz2 wk2) = k `LP.is_weaker_than` k'
@@ -47,53 +85,141 @@ let is_weaker_than_glb #nz1 #wk1 (k1:parser_kind nz1 wk1)
              [SMTPat (is_weaker_than (glb k1 k2) k2)]]]
   = ()
 
-/// Parser: return
-inline_for_extraction noextract
-let parse_ret #t (v:t)
-  : Tot (parser ret_kind t)
-  = LPC.parse_ret #t v
+let full_parse_dep_pair_body_parser
+  (#t1: Type)
+  (#nz2:_) (#wk2: _) (#k2:parser_kind nz2 wk2) (#t2: (t1 -> Tot Type)) (p2: (x: t1) -> full_parser k2 (t2 x))
+  (x: t1)
+: LP.parser k2 (t2 x)
+= (p2 x).pf_parser
+
+let full_parse_dep_pair_body_serializer
+  (#t1: Type)
+  (#nz2:_) (#wk2: _) (#k2:parser_kind nz2 wk2) (#t2: (t1 -> Tot Type)) (p2: (x: t1) -> full_parser k2 (t2 x))
+  (x: t1)
+: LP.serializer (full_parse_dep_pair_body_parser p2 x)
+= (p2 x).pf_serializer
 
 /// Parser: bind
 inline_for_extraction noextract
-let parse_dep_pair p1 p2
-  = LPC.parse_dtuple2 p1 p2
+let full_parse_dep_pair (#nz1:_) (#k1:parser_kind nz1 WeakKindStrongPrefix) (#t1: Type) (p1: full_parser k1 t1)
+                   (#nz2:_) (#wk2: _) (#k2:parser_kind nz2 wk2) (#t2: (t1 -> Tot Type)) (p2: (x: t1) -> full_parser k2 (t2 x))
+  : Tot (full_parser (and_then_kind k1 k2) (dtuple2 t1 t2) )
+  = {
+    pf_parser = LPC.parse_dtuple2 p1.pf_parser (full_parse_dep_pair_body_parser p2);
+    pf_serializer = LPC.serialize_dtuple2 p1.pf_serializer (full_parse_dep_pair_body_serializer p2);
+  }
+
+let parse_dep_pair_body_serializable
+  (#t1: Type)
+  (#nz2:_) (#wk2: _) (#k2:parser_kind nz2 wk2) (#t2: (t1 -> Tot Type)) (p2: (x: t1) -> parser k2 (t2 x))
+  (x1: t1)
+: Tot (t2 x1 -> GTot bool)
+= (p2 x1).p_serializable
+
+let parse_dep_pair_body_type
+  (#t1: Type)
+  (#nz2:_) (#wk2: _) (#k2:parser_kind nz2 wk2) (#t2: (t1 -> Tot Type)) (p2: (x: t1) -> parser k2 (t2 x))
+  (x1: t1)
+= LPC.parse_filter_refine (parse_dep_pair_body_serializable p2 x1)
+
+let parse_dep_pair_body_full_parser
+  (#t1: Type)
+  (#nz2:_) (#wk2: _) (#k2:parser_kind nz2 wk2) (#t2: (t1 -> Tot Type)) (p2: (x: t1) -> parser k2 (t2 x))
+  (x1: t1)
+: full_parser k2 (parse_dep_pair_body_type p2 x1)
+= (p2 x1).p_full_parser
+
+let parse_dep_pair_serializable
+  (#nz1:_) (#k1:parser_kind nz1 WeakKindStrongPrefix) (#t1: Type) (p1: parser k1 t1)
+                   (#nz2:_) (#wk2: _) (#k2:parser_kind nz2 wk2) (#t2: (t1 -> Tot Type)) (p2: (x: t1) -> parser k2 (t2 x))
+  (x: dtuple2 t1 t2)
+: GTot bool
+= p1.p_serializable (dfst x) && (p2 (dfst x)).p_serializable (dsnd x)
+
+inline_for_extraction noextract
+let parse_dep_pair #_ #_ #t1 p1 #_ #_ #_ #t2 p2 =
+  mk_parser_gen
+    (full_parse_dep_pair p1.p_full_parser (parse_dep_pair_body_full_parser p2))
+    (parse_dep_pair_serializable p1 p2)
+    (fun (| x1, x2 |) -> (| (x1 <: t1) , (x2 <: t2 x1) |))
+    (fun (x: LPC.parse_filter_refine (parse_dep_pair_serializable p1 p2)) -> (| dfst x, dsnd x |))
 
 /// Parser: sequencing
 inline_for_extraction noextract
-let parse_pair p1 p2
-  = LPC.nondep_then p1 p2
+let full_parse_pair (#nz1:_) (#k1:parser_kind nz1 WeakKindStrongPrefix) (#t1:_) (p1:full_parser k1 t1)
+               (#nz2:_) (#wk2: _) (#k2:parser_kind nz2 wk2) (#t2:_) (p2:full_parser k2 t2)
+  : Tot (full_parser (and_then_kind k1 k2) (t1 * t2))
+  = {
+    pf_parser = LPC.nondep_then p1.pf_parser p2.pf_parser;
+    pf_serializer = LPC.serialize_nondep_then p1.pf_serializer p2.pf_serializer;
+  }
+
+inline_for_extraction noextract
+let parse_pair_serializable (#nz1:_) (#k1:parser_kind nz1 WeakKindStrongPrefix) (#t1:_) (p1:parser k1 t1)
+               (#nz2:_) (#wk2: _) (#k2:parser_kind nz2 wk2) (#t2:_) (p2:parser k2 t2)
+    (x: (t1 & t2))
+  : GTot bool
+= p1.p_serializable (fst x) && p2.p_serializable (snd x)
+
+inline_for_extraction noextract
+let parse_pair #_ #_ #t1 p1 #_ #_ #_ #t2 p2
+  = mk_parser_gen
+      (full_parse_pair p1.p_full_parser p2.p_full_parser)
+      (parse_pair_serializable p1 p2)
+      (fun x -> ((fst x <: t1), (snd x <: t2)))
+      (fun (x: LPC.parse_filter_refine (parse_pair_serializable p1 p2)) -> (fst x, snd x))
 
 /// Parser: map
 let injective_map a b = (a -> Tot b) //{LPC.synth_injective f}
 
 inline_for_extraction noextract
+let full_parse_filter (#nz:_) (#wk: _) (#k:parser_kind nz wk) (#t:_) (p:full_parser k t) (f:(t -> bool))
+  : Tot (full_parser (filter_kind k) (refine t f))
+  = {
+  pf_parser = LPC.parse_filter p.pf_parser f;
+  pf_serializer = LPC.serialize_filter p.pf_serializer f;
+}
+
+inline_for_extraction noextract
 let parse_filter p f
-  = LPC.parse_filter p f
+= mk_parser_gen
+    (full_parse_filter p.p_full_parser f)
+    p.p_serializable
+    (fun x -> x)
+    (fun x -> x)
 
 /// Parser: weakening kinds
 inline_for_extraction noextract
 let parse_weaken #nz #wk (#k:parser_kind nz wk) #t (p:parser k t)
                  #nz' #wk' (k':parser_kind nz' wk' {k' `is_weaker_than` k})
   : Tot (parser k' t)
-  = LP.weaken k' p
+  = {
+  p_serializable = p.p_serializable;
+  p_full_parser = {
+    pf_parser = LP.weaken k' p.p_full_parser.pf_parser;
+    pf_serializer = LPC.serialize_weaken k' p.p_full_parser.pf_serializer;
+  }
+}
 
 /// Parser: weakening kinds
 inline_for_extraction noextract
 let parse_weaken_left #nz #wk #k p k'
-  = LP.weaken (glb k' k) p
+  = parse_weaken p (glb k' k)
 
 /// Parser: weakening kinds
 inline_for_extraction noextract
 let parse_weaken_right #nz #wk #k p k'
-  = LP.weaken (glb k k') p
+  = parse_weaken p (glb k k')
 
 /// Parser: unreachable, for default cases of exhaustive pattern matching
 inline_for_extraction noextract
 let parse_impos ()
   : parser impos_kind False
-  = let p : LP.bare_parser False = fun b -> None in
-    LP.parser_kind_prop_equiv impos_kind p;
-    p
+= mk_parser
+  {
+      pf_parser = LPC.fail_parser impos_kind False;
+      pf_serializer = LPC.fail_serializer impos_kind False (fun _ -> ());
+  }
 
 let parse_ite e p1 p2
   = if e then p1 () else p2 ()
@@ -101,19 +227,18 @@ let parse_ite e p1 p2
 let nlist (n:U32.t) (t:Type) = list t
 
 inline_for_extraction noextract
-let parse_nlist'
+let parse_nlist1
         (n:U32.t)
-        (n_const:option nat { Some? n_const ==> Some?.v n_const == U32.v n })
         (#wk: _)
         (#k:parser_kind true wk)
         (#t:_)
-        (p:parser k t)
-  : Tot (LP.bare_parser (nlist n t))
+        (p:LP.parser k t)
+  : Tot (LP.parser _ (nlist n t))
   = LowParse.Spec.FLData.parse_fldata (LowParse.Spec.List.parse_list p) (U32.v n)
 
 let parse_nlist_total_fixed_size_aux
-  (n:U32.t) (n_is_const:option nat { memoizes_n_as_const n_is_const n })
-  (#wk: _) (#k:parser_kind true wk) #t (p:parser k t)
+  (n:U32.t)
+  (#wk: _) (#k:parser_kind true wk) #t (p:LP.parser k t)
   (x: LP.bytes)
 : Lemma
   (requires (
@@ -125,7 +250,7 @@ let parse_nlist_total_fixed_size_aux
     Seq.length x >= U32.v n
   ))
   (ensures (
-    Some? (LP.parse (parse_nlist' n n_is_const p) x)
+    Some? (LP.parse (parse_nlist1 n p) x)
   ))
 = let x' = Seq.slice x 0 (U32.v n) in
   let cnt = (U32.v n / k.LP.parser_kind_low) in
@@ -134,9 +259,31 @@ let parse_nlist_total_fixed_size_aux
   LowParse.Spec.List.parse_list_total_constant_size p cnt x';
   LP.parser_kind_prop_equiv LowParse.Spec.List.parse_list_kind (LowParse.Spec.List.parse_list p)
 
-let parse_nlist_total_fixed_size_kind_correct
+inline_for_extraction noextract
+let parse_nlist2
+        (n:U32.t)
+        (#k:parser_kind true WeakKindStrongPrefix)
+        (#t:_)
+        (#p:LP.parser k t)
+        (s: LP.serializer p)
+  = LowParse.Spec.FLData.parse_fldata_strong (LowParse.Spec.List.serialize_list _ s) (U32.v n)
+
+inline_for_extraction noextract
+let serialize_nlist2
+        (n:U32.t)
+        (#k:parser_kind true WeakKindStrongPrefix)
+        (#t:_)
+        (#p:LP.parser k t)
+        (s: LP.serializer p)
+: Tot (LP.serializer (parse_nlist2 n s))
+= LowParse.Spec.FLData.serialize_fldata_strong (LowParse.Spec.List.serialize_list _ s) (U32.v n)
+
+let parse_nlist_total_fixed_size_kind_correct2
   (n:U32.t) (n_is_const:option nat { memoizes_n_as_const n_is_const n })
-  (#wk: _) (#k:parser_kind true wk) #t (p:parser k t)
+        (#k:parser_kind true WeakKindStrongPrefix)
+        (#t:_)
+        (#p:LP.parser k t)
+        (s: LP.serializer p)
 : Lemma
   (requires (
     let open LP in
@@ -146,22 +293,316 @@ let parse_nlist_total_fixed_size_kind_correct
     k.parser_kind_metadata == Some ParserKindMetadataTotal
   ))
   (ensures (
-    LP.parser_kind_prop (LP.total_constant_size_parser_kind (U32.v n)) (parse_nlist' n n_is_const p) /\
+    LP.parser_kind_prop (LP.total_constant_size_parser_kind (U32.v n)) (parse_nlist2 n s) /\
     (Some? n_is_const ==> kind_nlist k n_is_const == LP.total_constant_size_parser_kind (U32.v n))
   ))
-= LP.parser_kind_prop_equiv (LowParse.Spec.FLData.parse_fldata_kind (U32.v n) LowParse.Spec.List.parse_list_kind) (parse_nlist' n n_is_const p);
-  LP.parser_kind_prop_equiv (LP.total_constant_size_parser_kind (U32.v n)) (parse_nlist' n n_is_const p);
-  Classical.forall_intro (Classical.move_requires (parse_nlist_total_fixed_size_aux n n_is_const p))
+= LP.parser_kind_prop_equiv (LowParse.Spec.FLData.parse_fldata_kind (U32.v n) LowParse.Spec.List.parse_list_kind) (parse_nlist2 n s);
+  LP.parser_kind_prop_equiv (LP.total_constant_size_parser_kind (U32.v n)) (parse_nlist2 n s);
+  Classical.forall_intro (Classical.move_requires (parse_nlist_total_fixed_size_aux n p))
 
 inline_for_extraction noextract
-let parse_nlist n n_is_const #wk #k #t p
+let parse_nlist3
+        (n:U32.t)
+        (n_const:option nat { Some? n_const ==> Some?.v n_const == U32.v n })
+        (#k:parser_kind true WeakKindStrongPrefix)
+        (#t:_)
+        (#p:LP.parser k t)
+        (s: LP.serializer p)
+  : Tot (LP.parser (kind_nlist k n_const) (LowParse.Spec.FLData.parse_fldata_strong_t (LowParse.Spec.List.serialize_list _ s) (U32.v n)))
   = let open LowParse.Spec.FLData in
     let open LowParse.Spec.List in
-    let p' = parse_nlist' n n_is_const p in
+    let p' : bare_parser (LowParse.Spec.FLData.parse_fldata_strong_t (LowParse.Spec.List.serialize_list _ s) (U32.v n)) = parse_nlist2 n s in
     LP.parser_kind_prop_equiv (parse_fldata_kind (U32.v n) (parse_list_kind)) p';
-    LP.parser_kind_prop_equiv (kind_nlist k n_is_const) p';
-    Classical.move_requires (parse_nlist_total_fixed_size_kind_correct n n_is_const #wk #k #t) p;
+    LP.parser_kind_prop_equiv (kind_nlist k n_const) p';
+    Classical.move_requires (parse_nlist_total_fixed_size_kind_correct2 n n_const #k #t #p) s;
     p'
+
+inline_for_extraction noextract
+let serialize_nlist3
+        (n:U32.t)
+        (n_const:option nat { Some? n_const ==> Some?.v n_const == U32.v n })
+        (#k:parser_kind true WeakKindStrongPrefix)
+        (#t:_)
+        (#p:LP.parser k t)
+        (s: LP.serializer p)
+  : Tot (LP.serializer (parse_nlist3 n n_const s))
+= LP.serialize_ext _ (serialize_nlist2 n s) (parse_nlist3 n n_const s)
+
+let parse_nlist_total_fixed_size_kind_correct3
+  (n:U32.t) (n_is_const:option nat { memoizes_n_as_const n_is_const n })
+  (#k:parser_kind true WeakKindStrongPrefix) #t (#p:LP.parser k t) (s: LP.serializer p)
+: Lemma
+  (requires (
+    let open LP in
+    k.parser_kind_subkind == Some ParserStrong /\
+    k.parser_kind_high == Some k.parser_kind_low /\
+    U32.v n % k.parser_kind_low == 0 /\
+    k.parser_kind_metadata == Some ParserKindMetadataTotal
+  ))
+  (ensures (
+    LP.parser_kind_prop (LP.total_constant_size_parser_kind (U32.v n)) (parse_nlist3 n n_is_const s) /\
+    (Some? n_is_const ==> kind_nlist k n_is_const == LP.total_constant_size_parser_kind (U32.v n))
+  ))
+= parse_nlist_total_fixed_size_kind_correct2 n n_is_const s;
+  LP.parser_kind_prop_equiv (LP.total_constant_size_parser_kind (U32.v n)) (parse_nlist2 n s);
+  LP.parser_kind_prop_equiv (LP.total_constant_size_parser_kind (U32.v n)) (parse_nlist3 n n_is_const s);
+  ()
+
+let rec list_ghost_for_all
+  (#t: Type)
+  (f: t -> GTot bool)
+  (l: list t)
+: GTot bool
+= match l with
+  | [] -> true
+  | a :: q -> if f a then list_ghost_for_all f q else false
+
+let list_ghost_for_all'
+  (#t: Type)
+  (f: t -> GTot bool)
+  (l: list t)
+: GTot bool
+= match l with
+  | [] -> true
+  | a :: q -> if f a then list_ghost_for_all f q else false
+
+let list_ghost_for_all_unfold
+  (#t: Type)
+  (f: t -> GTot bool)
+  (l: list t)
+: Lemma
+  (list_ghost_for_all f l == list_ghost_for_all' f l)
+= assert_norm (list_ghost_for_all f l == list_ghost_for_all' f l)
+
+let rec list_ghost_for_all_pull_refine
+  (#t: Type)
+  (f: t -> GTot bool)
+  (l: list (LPC.parse_filter_refine f))
+: GTot (LPC.parse_filter_refine (list_ghost_for_all f))
+= match l with
+  | [] -> list_ghost_for_all_unfold f []; []
+  | a :: q ->
+    let l' : list t = a :: list_ghost_for_all_pull_refine f q in
+    list_ghost_for_all_unfold f l';
+    l'
+
+let list_ghost_for_all_pull_refine'
+  (#t: Type)
+  (f: t -> GTot bool)
+  (l: list (LPC.parse_filter_refine f))
+: GTot (list t)
+= match l with
+  | [] -> []
+  | a :: q -> a :: list_ghost_for_all_pull_refine f q
+
+let list_ghost_for_all_pull_refine_unfold
+  (#t: Type)
+  (f: t -> GTot bool)
+  (l: list (LPC.parse_filter_refine f))
+: Lemma
+  (list_ghost_for_all_pull_refine f l == list_ghost_for_all_pull_refine' f l)
+= assert_norm (list_ghost_for_all_pull_refine f l == list_ghost_for_all_pull_refine' f l)
+
+let rec list_ghost_for_all_push_refine
+  (#t: Type)
+  (f: t -> GTot bool)
+  (l: LPC.parse_filter_refine (list_ghost_for_all f))
+: GTot (list (LPC.parse_filter_refine f))
+= list_ghost_for_all_unfold f l;
+  match l with
+  | [] -> []
+  | a :: q ->
+    a :: list_ghost_for_all_push_refine f q
+
+let list_ghost_for_all_push_refine'
+  (#t: Type)
+  (f: t -> GTot bool)
+  (l: LPC.parse_filter_refine (list_ghost_for_all f))
+: GTot (list (LPC.parse_filter_refine f))
+= list_ghost_for_all_unfold f l;
+  match l with
+  | [] -> []
+  | a :: q -> a :: list_ghost_for_all_push_refine f q
+
+let list_ghost_for_all_push_refine_unfold
+  (#t: Type)
+  (f: t -> GTot bool)
+  (l: LPC.parse_filter_refine (list_ghost_for_all f))
+: Lemma
+  (list_ghost_for_all_push_refine f l == list_ghost_for_all_push_refine' f l)
+= assert_norm (list_ghost_for_all_push_refine f l == list_ghost_for_all_push_refine' f l)
+
+let rec synth_inverse_list_ghost_for_all_pull_push_refine'
+  (#t: Type)
+  (f: t -> GTot bool)
+  (l: LPC.parse_filter_refine (list_ghost_for_all f))
+: Lemma
+  (ensures (list_ghost_for_all_pull_refine f (list_ghost_for_all_push_refine f l) == l))
+  (decreases l)
+= list_ghost_for_all_pull_refine_unfold f (list_ghost_for_all_push_refine f l);
+  list_ghost_for_all_push_refine_unfold f l;
+  list_ghost_for_all_unfold f l;
+  match l with
+  | [] -> ()
+  | a :: q -> synth_inverse_list_ghost_for_all_pull_push_refine' f q
+
+let synth_inverse_list_ghost_for_all_pull_push_refine
+  (#t: Type)
+  (f: t -> GTot bool)
+: Lemma
+  (ensures (LPC.synth_inverse (list_ghost_for_all_pull_refine f) (list_ghost_for_all_push_refine f)))
+  [SMTPat (list_ghost_for_all_pull_refine f)]
+= LPC.synth_inverse_intro' (list_ghost_for_all_pull_refine f) (list_ghost_for_all_push_refine f) (synth_inverse_list_ghost_for_all_pull_push_refine' f)
+
+let rec synth_inverse_list_ghost_for_all_push_pull_refine'
+  (#t: Type)
+  (f: t -> GTot bool)
+  (l: list (LPC.parse_filter_refine f))
+: Lemma
+  (ensures (list_ghost_for_all_push_refine f (list_ghost_for_all_pull_refine f l) == l))
+  (decreases l)
+= list_ghost_for_all_push_refine_unfold f (list_ghost_for_all_pull_refine f l);
+  list_ghost_for_all_pull_refine_unfold f l;
+  list_ghost_for_all_unfold f (list_ghost_for_all_pull_refine f l);
+  match l with
+  | [] -> ()
+  | a :: q -> synth_inverse_list_ghost_for_all_push_pull_refine' f q
+
+let synth_inverse_list_ghost_for_all_push_pull_refine
+  (#t: Type)
+  (f: t -> GTot bool)
+: Lemma
+  (ensures (LPC.synth_inverse (list_ghost_for_all_push_refine f) (list_ghost_for_all_pull_refine f)))
+  [SMTPat (list_ghost_for_all_pull_refine f)]
+= LPC.synth_inverse_intro' (list_ghost_for_all_push_refine f) (list_ghost_for_all_pull_refine f) (synth_inverse_list_ghost_for_all_push_pull_refine' f)
+
+let parse_nlist_serializable
+    (n:U32.t)
+    (#k:parser_kind true WeakKindStrongPrefix)
+    (#t:_)
+    (#f: (t -> GTot bool))
+    (#p:LP.parser k (LPC.parse_filter_refine f))
+    (s: LP.serializer p)
+    (l: list t)
+: GTot bool
+= list_ghost_for_all f l &&
+  Seq.length (LP.serialize (LowParse.Spec.List.serialize_list _ s) (list_ghost_for_all_push_refine f l)) = U32.v n
+
+let parse_nlist_synth_intro
+    (n:U32.t)
+    (#k:parser_kind true WeakKindStrongPrefix)
+    (#t:_)
+    (#f: (t -> GTot bool))
+    (#p:LP.parser k (LPC.parse_filter_refine f))
+    (s: LP.serializer p)
+    (l: LowParse.Spec.FLData.parse_fldata_strong_t (LowParse.Spec.List.serialize_list _ s) (U32.v n))
+: GTot (LPC.parse_filter_refine (parse_nlist_serializable n s))
+= synth_inverse_list_ghost_for_all_push_pull_refine f;
+  list_ghost_for_all_pull_refine f l
+
+let parse_nlist_synth_intro_injective
+    (n:U32.t)
+    (#k:parser_kind true WeakKindStrongPrefix)
+    (#t:_)
+    (#f: (t -> GTot bool))
+    (#p:LP.parser k (LPC.parse_filter_refine f))
+    (s: LP.serializer p)
+: Lemma
+  (ensures (LPC.synth_injective (parse_nlist_synth_intro n s)))
+  [SMTPat (parse_nlist_synth_intro n s)]
+= synth_inverse_list_ghost_for_all_pull_push_refine f;
+  synth_inverse_list_ghost_for_all_push_pull_refine f
+
+inline_for_extraction noextract
+let parse_nlist4
+        (n:U32.t)
+        (n_const:option nat { Some? n_const ==> Some?.v n_const == U32.v n })
+        (#k:parser_kind true WeakKindStrongPrefix)
+        (#t:_)
+        (#f: (t -> GTot bool))
+        (#p:LP.parser k (LPC.parse_filter_refine f))
+        (s: LP.serializer p)
+  : Tot (LP.parser (kind_nlist k n_const) (LPC.parse_filter_refine (parse_nlist_serializable n s)))
+= LPC.parse_synth
+    (parse_nlist3 n n_const s)
+    (parse_nlist_synth_intro n s)
+
+let parse_nlist_synth_elim
+    (n:U32.t)
+    (#k:parser_kind true WeakKindStrongPrefix)
+    (#t:_)
+    (#f: (t -> GTot bool))
+    (#p:LP.parser k (LPC.parse_filter_refine f))
+    (s: LP.serializer p)
+    (l: LPC.parse_filter_refine (parse_nlist_serializable n s))
+: GTot (LowParse.Spec.FLData.parse_fldata_strong_t (LowParse.Spec.List.serialize_list _ s) (U32.v n))
+= synth_inverse_list_ghost_for_all_push_pull_refine f;
+  list_ghost_for_all_push_refine f l
+
+let parse_nlist_synth_intro_inverse
+    (n:U32.t)
+    (#k:parser_kind true WeakKindStrongPrefix)
+    (#t:_)
+    (#f: (t -> GTot bool))
+    (#p:LP.parser k (LPC.parse_filter_refine f))
+    (s: LP.serializer p)
+: Lemma
+  (ensures (LPC.synth_inverse (parse_nlist_synth_intro n s) (parse_nlist_synth_elim n s)))
+  [SMTPat (parse_nlist_synth_intro n s)]
+= synth_inverse_list_ghost_for_all_pull_push_refine f;
+  synth_inverse_list_ghost_for_all_push_pull_refine f
+
+inline_for_extraction noextract
+let serialize_nlist4
+        (n:U32.t)
+        (n_const:option nat { Some? n_const ==> Some?.v n_const == U32.v n })
+        (#k:parser_kind true WeakKindStrongPrefix)
+        (#t:_)
+        (#f: (t -> GTot bool))
+        (#p:LP.parser k (LPC.parse_filter_refine f))
+        (s: LP.serializer p)
+  : Tot (LP.serializer (parse_nlist4 n n_const s))
+= LPC.serialize_synth
+    (parse_nlist3 n n_const s)
+    (parse_nlist_synth_intro n s)
+    (serialize_nlist3 n n_const s)
+    (parse_nlist_synth_elim n s)
+    ()
+
+inline_for_extraction noextract
+let parse_nlist n n_is_const #k #t p
+  = {
+    p_serializable = parse_nlist_serializable n p.p_full_parser.pf_serializer;
+    p_full_parser = {
+      pf_parser = parse_nlist4 n n_is_const p.p_full_parser.pf_serializer;
+      pf_serializer = serialize_nlist4 n n_is_const p.p_full_parser.pf_serializer;
+    }
+  }
+
+let parse_nlist_total_fixed_size_kind_correct
+  (n:U32.t) (n_is_const:option nat { memoizes_n_as_const n_is_const n })
+  (#k:parser_kind true WeakKindStrongPrefix) #t (p:parser k t)
+: Lemma
+  (requires (
+    let open LP in
+    k.parser_kind_subkind == Some ParserStrong /\
+    k.parser_kind_high == Some k.parser_kind_low /\
+    U32.v n % k.parser_kind_low == 0 /\
+    k.parser_kind_metadata == Some ParserKindMetadataTotal
+  ))
+  (ensures (
+    LP.parser_kind_prop (LP.total_constant_size_parser_kind (U32.v n)) (parse_nlist n n_is_const p).p_full_parser.pf_parser /\
+    (Some? n_is_const ==> kind_nlist k n_is_const == LP.total_constant_size_parser_kind (U32.v n))
+  ))
+= let s = p.p_full_parser.pf_serializer in
+  parse_nlist_total_fixed_size_kind_correct3 n n_is_const s;
+  Classical.forall_intro (LPC.parse_synth_eq2 (parse_nlist3 n n_is_const s) (parse_nlist_synth_intro n s) ());
+  LP.parser_kind_prop_equiv (LP.total_constant_size_parser_kind (U32.v n)) (parse_nlist3 n n_is_const s);
+  let pl : LP.parser (LP.total_constant_size_parser_kind (U32.v n)) (LowParse.Spec.FLData.parse_fldata_strong_t (LowParse.Spec.List.serialize_list _ s) (U32.v n)) = (parse_nlist3 n n_is_const s <: LP.bare_parser _) in
+  Classical.forall_intro (LPC.parse_synth_eq2 (parse_nlist3 n n_is_const s) (parse_nlist_synth_intro n s) ());
+  Classical.forall_intro (LPC.parse_synth_eq2 pl (parse_nlist_synth_intro n s) ());
+  LP.parser_kind_prop_ext (LP.total_constant_size_parser_kind (U32.v n)) (LPC.parse_synth pl (parse_nlist_synth_intro n s)) (parse_nlist n n_is_const p).p_full_parser.pf_parser;
+  ()
 
 let all_bytes = Seq.seq LP.byte
 let parse_all_bytes' 
@@ -328,9 +769,9 @@ let read____UINT32 = LowParse.Low.BoundedInt.read_u32_le
 let parse____UINT64 = LowParse.Spec.Int.parse_u64_le
 let read____UINT64 = LowParse.Low.Int.read_u64_le
   
-let parse_unit = parse_ret ()
+let parse_unit = LPC.parse_empty
 
 inline_for_extraction noextract
 let read_unit
-  : LPL.leaf_reader (parse_ret ())
+  : LPL.leaf_reader unit
   = LPLC.read_ret ()
